examples/hoare_logic/blocking_semantics5/blocking_semantics5_TypingAndSemantics_type_preservation_1.v
@@ -351,37 +351,27 @@ Definition compatible_env(sigma:(map mident value)) (sigmat:(map mident
   id)) = (get sigmat id))) /\ forall (id:ident), ((type_value (get_stack id
   pi)) = (get_vartype id pit)).
 
-Require Import Why3.
+Axiom eval_type_term : forall (t:term) (sigma:(map mident value)) (pi:(list
+  (ident* value)%type)) (sigmat:(map mident datatype)) (pit:(list (ident*
+  datatype)%type)) (ty:datatype), (compatible_env sigma sigmat pi pit) ->
+  ((type_term sigmat pit t ty) -> ((type_value (eval_term sigma pi
+  t)) = ty)).
 
+Require Import Why3.
 Ltac ae := why3 "alt-ergo" timelimit 3.
 
 (* Why3 goal *)
-Theorem eval_type_term : forall (t:term),
-  match t with
-  | (Tvalue v) => True
-  | (Tvar i) => True
-  | (Tderef m) => True
-  | (Tbin t1 o t2) => (forall (sigma:(map mident value)) (pi:(list (ident*
-      value)%type)) (sigmat:(map mident datatype)) (pit:(list (ident*
-      datatype)%type)) (ty:datatype), (compatible_env sigma sigmat pi pit) ->
-      ((type_term sigmat pit t2 ty) -> ((type_value (eval_term sigma pi
-      t2)) = ty))) -> ((forall (sigma:(map mident value)) (pi:(list (ident*
-      value)%type)) (sigmat:(map mident datatype)) (pit:(list (ident*
-      datatype)%type)) (ty:datatype), (compatible_env sigma sigmat pi pit) ->
-      ((type_term sigmat pit t1 ty) -> ((type_value (eval_term sigma pi
-      t1)) = ty))) -> forall (sigma:(map mident value)) (pi:(list (ident*
-      value)%type)) (sigmat:(map mident datatype)) (pit:(list (ident*
-      datatype)%type)) (ty:datatype), (compatible_env sigma sigmat pi pit) ->
-      ((type_term sigmat pit t ty) -> ((type_value (eval_term sigma pi
-      t)) = ty)))
-  end.
-destruct t; auto.
-simpl.
-intros.
-inversion H2; subst; clear H2.
-generalize (type_inversion (eval_term sigma pi t1)).
-generalize (type_inversion (eval_term sigma pi t2)).
-destruct H11; ae.
+Theorem type_preservation : forall (s1:stmt) (s2:stmt) (sigma1:(map mident
+  value)) (sigma2:(map mident value)) (pi1:(list (ident* value)%type))
+  (pi2:(list (ident* value)%type)) (sigmat:(map mident datatype)) (pit:(list
+  (ident* datatype)%type)), ((type_stmt sigmat pit s1) /\
+  ((compatible_env sigma1 sigmat pi1 pit) /\ (one_step sigma1 pi1 s1 sigma2
+  pi2 s2))) -> ((type_stmt sigmat pit s2) /\ (compatible_env sigma2 sigmat
+  pi2 pit)).
+intros s1 s2 sigma1 sigma2 pi1 pi2 sigmat pit (h1,(h2,h3)).
+induction h3; try ae.
+inversion h1; subst; clear h1.
+ae.
 Qed.
 
 
